hax-lib/proof-libs/fstar/rust_primitives/64bit/Rust_primitives.SizeBits.fst
@@ -1,0 +1,3 @@
+module Rust_primitives.SizeBits
+
+let size_bits: n:nat{n == 32 \/ n == 64} = 64
