hax-lib/proof-libs/fstar/rust_primitives/Rust_primitives.Arrays.fst
@@ -1,0 +1,106 @@
+module Rust_primitives.Arrays
+
+open Rust_primitives.Integers
+open FStar.Mul
+open FStar.List.Tot.Properties
+
+#set-options "--fuel 1 --ifuel 0 --z3rlimit 30"
+
+let rec list_create (#a: Type) (n: nat) (x: a): Tot (l:list a{FStar.List.Tot.length l == n}) (decreases n)
+  = if n = 0 then []
+    else x :: list_create (n-1) x
+
+let rec list_init (#a: Type) (n: nat) (f: (i:nat{i < n}) -> a): Tot (l:list a{FStar.List.Tot.length l == n}) (decreases n)
+  = if n = 0 then []
+    else f 0 :: list_init (n-1) (fun (i:nat{i < n-1}) -> f (i+1))
+
+let rec list_slice (#a: Type) (l: list a) (i: nat) (j: nat{i <= j /\ j <= FStar.List.Tot.length l}):
+  Tot (r:list a{FStar.List.Tot.length r == j - i}) (decreases (j - i))
+  = if i = j then []
+    else FStar.List.Tot.index l i :: list_slice l (i+1) j
+
+let rec list_upd (#a: Type) (l: list a) (i: nat{i < FStar.List.Tot.length l}) (x: a):
+  Tot (r:list a{FStar.List.Tot.length r == FStar.List.Tot.length l}) (decreases i)
+  = match l with
+    | hd :: tl -> if i = 0 then x :: tl else hd :: list_upd tl (i-1) x
+
+let map_array (#a #b: Type) #n (arr: t_Array a n) (f: a -> b): t_Array b n
+  = list_init (v n) (fun i -> f (FStar.List.Tot.index arr i))
+
+let createi #t (l:usize) (f:(u:usize{u <. l} -> t))
+    : Pure (t_Array t l)
+      (requires True)
+      (ensures (fun res -> (forall i. FStar.List.Tot.index res (v i) == f i)))
+  = admit (); // TODO: prove the ensures
+    list_init (v l) (fun i -> f (sz i))
+
+#push-options "--fuel 2 --z3rlimit 60"
+
+let lemma_index_concat #t (x:t_Slice t) (y:t_Slice t{range (v (length x) + v (length y)) usize_inttype}) (i:usize{i <. length x +! length y}):
+           Lemma (if i <. length x then
+                    FStar.List.Tot.index (concat x y) (v i) == FStar.List.Tot.index x (v i)
+                  else
+                    FStar.List.Tot.index (concat x y) (v i) == FStar.List.Tot.index y (v (i -! length x)))
+           [SMTPat (FStar.List.Tot.index (concat #t x y) (v i))]
+  = admit () // TODO: prove via induction on x
+
+let rec lemma_index_list_slice (#a: Type) (l: list a) (i: nat) (j: nat{i <= j /\ j <= FStar.List.Tot.length l}) (k: nat{k < j - i}):
+  Lemma (ensures FStar.List.Tot.index (list_slice l i j) k == FStar.List.Tot.index l (i + k))
+        (decreases (j - i))
+  = if k = 0 then ()
+    else lemma_index_list_slice l (i+1) j (k-1)
+
+let lemma_index_slice #t (x:t_Slice t) (i:usize{i <=. length x}) (j:usize{i <=. j /\ j <=. length x})
+                                (k:usize{k <. j -! i}):
+           Lemma (FStar.List.Tot.index (slice x i j) (v k) == FStar.List.Tot.index x (v (i +! k)))
+           [SMTPat (FStar.List.Tot.index (slice x i j) (v k))]
+  = lemma_index_list_slice x (v i) (v j) (v k)
+
+#pop-options
+
+let eq_intro #t (a : list t) (b:list t{FStar.List.Tot.length a == FStar.List.Tot.length b}):
+       Lemma
+       (requires forall i. {:pattern FStar.List.Tot.index a i; FStar.List.Tot.index b i}
+                      i < FStar.List.Tot.length a ==>
+                      FStar.List.Tot.index a i == FStar.List.Tot.index b i)
+       (ensures a == b)
+       [SMTPat (a == b)]
+  = admit () // TODO: prove by induction on lists
+
+let split #t (a:t_Slice t) (m:usize{m <=. length a}):
+       Pure (t_Array t m & t_Array t (length a -! m))
+       True (ensures (fun (x,y) ->
+         x == slice a (sz 0) m /\
+         y == slice a m (length a) /\
+         concat #t x y == a))
+  = admit (); // TODO
+    let x = list_slice a 0 (v m) in
+    let y = list_slice a (v m) (FStar.List.Tot.length a) in
+    (x, y)
+
+let lemma_slice_append #t (x:t_Slice t) (y:t_Slice t) (z:t_Slice t):
+  Lemma (requires (range (v (length y) + v (length z)) usize_inttype /\
+                   length y +! length z == length x /\
+                   y == slice x (sz 0) (length y) /\
+                   z == slice x (length y) (length x)))
+        (ensures (x == concat y z))
+  = admit () // TODO
+
+let lemma_slice_append_3 #t (x:t_Slice t) (y:t_Slice t) (z:t_Slice t) (w:t_Slice t):
+  Lemma (requires (range (v (length y) + v (length z) + v (length w)) usize_inttype /\
+                   length y +! length z +! length w == length x /\
+                   y == slice x (sz 0) (length y) /\
+                   z == slice x (length y) (length y +! length z) /\
+                   w == slice x (length y +! length z) (length x)))
+        (ensures (x == concat y (concat z w)))
+  = admit () // TODO
+
+let lemma_slice_append_4 #t (x y z w u:t_Slice t) :
+  Lemma (requires (range (v (length y) + v (length z) + v (length w) + v (length u)) usize_inttype /\
+                   length y +! length z +! length w +! length u == length x /\
+                   y == slice x (sz 0) (length y) /\
+                   z == slice x (length y) (length y +! length z) /\
+                   w == slice x (length y +! length z) (length y +! length z +! length w) /\
+                   u == slice x (length y +! length z +! length w) (length x)))
+        (ensures (x == concat y (concat z (concat w u))))
+  = admit () // TODO
