hax-lib/proof-libs/fstar/rust_primitives/Rust_primitives.Hax.Folds.fst
@@ -1,0 +1,123 @@
+module Rust_primitives.Hax.Folds
+
+open Rust_primitives
+open Core_models.Ops.Range
+open FStar.Mul
+
+#set-options "--fuel 1 --ifuel 1 --z3rlimit 60"
+
+let rec fold_enumerated_chunked_slice_aux
+  (#t: Type0) (#acc_t: Type0)
+  (chunk_size: usize {v chunk_size > 0})
+  (s: t_Slice t)
+  (inv: acc_t -> (i:usize{v i <= FStar.List.Tot.length s / v chunk_size}) -> Type0)
+  (acc: acc_t)
+  (f: ( acc:acc_t
+      -> item:(usize & t_Slice t) {
+        let (i, s_chunk) = item in
+          v i < FStar.List.Tot.length s / v chunk_size
+        /\ length s_chunk == chunk_size
+        /\ nth_chunk_of s s_chunk (v i)
+        /\ inv acc i
+      }
+      -> acc':acc_t {
+        inv acc' (fst item +! sz 1)
+      }
+      )
+  )
+  (i: nat {i <= FStar.List.Tot.length s / v chunk_size})
+  : Tot acc_t (decreases (FStar.List.Tot.length s / v chunk_size - i))
+  = if i = FStar.List.Tot.length s / v chunk_size then acc
+    else
+      let chunk = Rust_primitives.Arrays.list_slice s (v chunk_size * i) (v chunk_size * (i + 1)) in
+      assume (inv acc (sz i));
+      assume (nth_chunk_of s chunk i);
+      let acc' = f acc (sz i, chunk) in
+      fold_enumerated_chunked_slice_aux chunk_size s inv acc' f (i + 1)
+
+let fold_enumerated_chunked_slice #t #acc_t chunk_size s inv init f =
+  admit (); // postcondition: inv result (length s / chunk_size)
+  fold_enumerated_chunked_slice_aux chunk_size s inv init f 0
+
+let rec fold_chunked_slice_aux
+  (#t: Type0) (#acc_t: Type0)
+  (chunk_size: usize {v chunk_size > 0})
+  (s: t_Slice t)
+  (inv: acc_t -> (i:usize) -> Type0)
+  (acc: acc_t)
+  (f: ( acc:acc_t
+      -> item:(t_Slice t) {
+        length item == chunk_size /\
+        inv acc (sz 0)
+      }
+      -> acc':acc_t {
+        inv acc' (sz 0)
+      }
+      )
+  )
+  (i: nat {i <= FStar.List.Tot.length s / v chunk_size})
+  : Tot acc_t (decreases (FStar.List.Tot.length s / v chunk_size - i))
+  = if i = FStar.List.Tot.length s / v chunk_size then acc
+    else
+      let chunk = Rust_primitives.Arrays.list_slice s (v chunk_size * i) (v chunk_size * (i + 1)) in
+      assume (inv acc (sz 0));
+      let acc' = f acc chunk in
+      fold_chunked_slice_aux chunk_size s inv acc' f (i + 1)
+
+let fold_chunked_slice #t #acc_t chunk_size s inv init f =
+  admit (); // postcondition
+  fold_chunked_slice_aux chunk_size s inv init f 0
+
+let rec fold_enumerated_slice_aux
+  (#t: Type0) (#acc_t: Type0)
+  (s: t_Slice t)
+  (inv: acc_t -> (i:usize{v i <= v (length s)}) -> Type0)
+  (acc: acc_t)
+  (f: (acc:acc_t -> i:(usize & t) {v (fst i) < v (length s) /\ snd i == FStar.List.Tot.index s (v (fst i)) /\ inv acc  (fst i)}
+                 -> acc':acc_t    {v (fst i) < v (length s) /\ inv acc' (fst i)}))
+  (i: nat {i <= FStar.List.Tot.length s})
+  : Tot acc_t (decreases (FStar.List.Tot.length s - i))
+  = if i = FStar.List.Tot.length s then acc
+    else
+      let item = FStar.List.Tot.index s i in
+      assume (inv acc (sz i));
+      let acc' = f acc (sz i, item) in
+      fold_enumerated_slice_aux s inv acc' f (i + 1)
+
+let fold_enumerated_slice #t #acc_t s inv init f =
+  admit (); // postcondition
+  fold_enumerated_slice_aux s inv init f 0
+
+let fold_enumerated_slice_return #t #acc_t #ret s inv init f =
+  admit () // TODO: implement with early return support
+
+let rec fold_range_step_by_aux
+  (#acc_t: Type0) (#u: inttype)
+  (start: int_t u) (end_: int_t u)
+  (step: usize {v step > 0 /\ range (v end_ + v step) u})
+  (inv: acc_t -> (i:int_t u{fold_range_step_by_wf_index start end_ step false (v i)}) -> Type0)
+  (acc: acc_t)
+  (f: (acc:acc_t -> i:int_t u  {v i < v end_ - ((v end_ - 1 - v start) % v step) /\ fold_range_step_by_wf_index start end_ step true (v i) /\ inv acc i}
+                 -> acc':acc_t {(inv acc' (mk_int (v i + v step)))}))
+  (cur: int_t u {v cur >= v start /\ v cur <= v end_})
+  : Tot acc_t (decreases (v end_ - v cur))
+  = if v cur >= v end_ then acc
+    else begin
+      assume (fold_range_step_by_wf_index start end_ step true (v cur));
+      assume (inv acc cur);
+      assume (v cur < v end_ - ((v end_ - 1 - v start) % v step));
+      let acc' = f acc cur in
+      assume (Rust_primitives.Integers.range (v step) u);
+      let next = cur +! (mk_int #u (v step)) in
+      if v next >= v end_ then acc'
+      else fold_range_step_by_aux start end_ step inv acc' f next
+    end
+
+let fold_range_step_by #acc_t #u start end_ step inv init f =
+  admit (); // postcondition
+  if v start < v end_
+  then fold_range_step_by_aux start end_ step inv init f start
+  else init
+
+let fold_return #it #acc #ret #item (i: it) (init: acc) f =
+  admit () // TODO: implement generic fold with early return
