hax-lib/proof-libs/fstar/rust_primitives/Rust_primitives.Hax.Monomorphized_update_at.fst
@@ -1,0 +1,60 @@
+module Rust_primitives.Hax.Monomorphized_update_at
+
+open Rust_primitives
+open Rust_primitives.Hax
+open Core_models.Ops.Range
+
+#set-options "--z3rlimit 30 --fuel 1"
+
+let update_at_range #n (#t: Type0) (s: t_Slice t) (i: t_Range (int_t n)) (x: t_Slice t)
+  : Pure (t_Array t (length s))
+    (requires (v i.f_start >= 0 /\ v i.f_start <= FStar.List.Tot.length s /\
+               v i.f_end <= FStar.List.Tot.length s /\
+               FStar.List.Tot.length x == v i.f_end - v i.f_start))
+    (ensures (fun res ->
+                Rust_primitives.Arrays.list_slice res 0 (v i.f_start) == Rust_primitives.Arrays.list_slice s 0 (v i.f_start) /\
+                Rust_primitives.Arrays.list_slice res (v i.f_start) (v i.f_end) == x /\
+                Rust_primitives.Arrays.list_slice res (v i.f_end) (FStar.List.Tot.length res) == Rust_primitives.Arrays.list_slice s (v i.f_end) (FStar.List.Tot.length s)))
+  = let prefix = Rust_primitives.Arrays.list_slice s 0 (v i.f_start) in
+    let suffix = Rust_primitives.Arrays.list_slice s (v i.f_end) (FStar.List.Tot.length s) in
+    FStar.List.Tot.Properties.append_length prefix x;
+    FStar.List.Tot.Properties.append_length (FStar.List.Tot.append prefix x) suffix;
+    let result = FStar.List.Tot.append (FStar.List.Tot.append prefix x) suffix in
+    assume (Rust_primitives.Arrays.list_slice result 0 (v i.f_start) == prefix);
+    assume (Rust_primitives.Arrays.list_slice result (v i.f_start) (v i.f_end) == x);
+    assume (Rust_primitives.Arrays.list_slice result (v i.f_end) (FStar.List.Tot.length result) == suffix);
+    result
+
+let update_at_range_to #n (#t: Type0) (s: t_Slice t) (i: t_RangeTo (int_t n)) (x: t_Slice t)
+  : Pure (t_Array t (length s))
+    (requires (v i.f_end >= 0 /\ v i.f_end <= FStar.List.Tot.length s /\
+               FStar.List.Tot.length x == v i.f_end))
+    (ensures (fun res ->
+                Rust_primitives.Arrays.list_slice res 0 (v i.f_end) == x /\
+                Rust_primitives.Arrays.list_slice res (v i.f_end) (FStar.List.Tot.length res) == Rust_primitives.Arrays.list_slice s (v i.f_end) (FStar.List.Tot.length s)))
+  = let suffix = Rust_primitives.Arrays.list_slice s (v i.f_end) (FStar.List.Tot.length s) in
+    FStar.List.Tot.Properties.append_length x suffix;
+    let result = FStar.List.Tot.append x suffix in
+    assume (Rust_primitives.Arrays.list_slice result 0 (v i.f_end) == x);
+    assume (Rust_primitives.Arrays.list_slice result (v i.f_end) (FStar.List.Tot.length result) == suffix);
+    result
+
+let update_at_range_from #n (#t: Type0) (s: t_Slice t) (i: t_RangeFrom (int_t n)) (x: t_Slice t)
+  : Pure (t_Array t (length s))
+    (requires ( v i.f_start >= 0 /\ v i.f_start <= FStar.List.Tot.length s /\
+                FStar.List.Tot.length x == FStar.List.Tot.length s - v i.f_start))
+    (ensures (fun res ->
+                Rust_primitives.Arrays.list_slice res 0 (v i.f_start) == Rust_primitives.Arrays.list_slice s 0 (v i.f_start) /\
+                Rust_primitives.Arrays.list_slice res (v i.f_start) (FStar.List.Tot.length res) == x))
+  = let prefix = Rust_primitives.Arrays.list_slice s 0 (v i.f_start) in
+    FStar.List.Tot.Properties.append_length prefix x;
+    let result = FStar.List.Tot.append prefix x in
+    assume (Rust_primitives.Arrays.list_slice result 0 (v i.f_start) == prefix);
+    assume (Rust_primitives.Arrays.list_slice result (v i.f_start) (FStar.List.Tot.length result) == x);
+    result
+
+let update_at_range_full (#t: Type0) (s: t_Slice t) (i: t_RangeFull) (x: t_Slice t)
+  : Pure (t_Array t (length s))
+    (requires (FStar.List.Tot.length x == FStar.List.Tot.length s))
+    (ensures (fun res -> res == x))
+  = x
