hax-lib/proof-libs/fstar/rust_primitives/Rust_primitives.Hax.Monomorphized_update_at.fsti
@@ -10,10 +10,10 @@ open Core_models.Ops.Range
 let update_at_usize
   (#t: Type0)
   (s: t_Slice t)
-  (i: usize {v i < Seq.length s})
+  (i: usize {v i < FStar.List.Tot.length s})
   (x: t)
   : t_Array t (length s)
-  = Seq.upd #t s (v i) x
+  = Rust_primitives.Arrays.list_upd s (v i) x
 
 val update_at_range #n
   (#t: Type0)
@@ -21,13 +21,13 @@ val update_at_range #n
   (i: t_Range (int_t n))
   (x: t_Slice t)
   : Pure (t_Array t (length s))
-    (requires (v i.f_start >= 0 /\ v i.f_start <= Seq.length s /\
-               v i.f_end <= Seq.length s /\
-               Seq.length x == v i.f_end - v i.f_start))
+    (requires (v i.f_start >= 0 /\ v i.f_start <= FStar.List.Tot.length s /\
+               v i.f_end <= FStar.List.Tot.length s /\
+               FStar.List.Tot.length x == v i.f_end - v i.f_start))
     (ensures (fun res ->
-                Seq.slice res 0 (v i.f_start) == Seq.slice s 0 (v i.f_start) /\
-                Seq.slice res (v i.f_start) (v i.f_end) == x /\
-                Seq.slice res (v i.f_end) (Seq.length res) == Seq.slice s (v i.f_end) (Seq.length s)))
+                Rust_primitives.Arrays.list_slice res 0 (v i.f_start) == Rust_primitives.Arrays.list_slice s 0 (v i.f_start) /\
+                Rust_primitives.Arrays.list_slice res (v i.f_start) (v i.f_end) == x /\
+                Rust_primitives.Arrays.list_slice res (v i.f_end) (FStar.List.Tot.length res) == Rust_primitives.Arrays.list_slice s (v i.f_end) (FStar.List.Tot.length s)))
 
 val update_at_range_to #n
   (#t: Type0)
@@ -35,11 +35,11 @@ val update_at_range_to #n
   (i: t_RangeTo (int_t n))
   (x: t_Slice t)
   : Pure (t_Array t (length s))
-    (requires (v i.f_end >= 0 /\ v i.f_end <= Seq.length s /\
-               Seq.length x == v i.f_end))
+    (requires (v i.f_end >= 0 /\ v i.f_end <= FStar.List.Tot.length s /\
+               FStar.List.Tot.length x == v i.f_end))
     (ensures (fun res ->
-                Seq.slice res 0 (v i.f_end) == x /\
-                Seq.slice res (v i.f_end) (Seq.length res) == Seq.slice s (v i.f_end) (Seq.length s)))
+                Rust_primitives.Arrays.list_slice res 0 (v i.f_end) == x /\
+                Rust_primitives.Arrays.list_slice res (v i.f_end) (FStar.List.Tot.length res) == Rust_primitives.Arrays.list_slice s (v i.f_end) (FStar.List.Tot.length s)))
 
 val update_at_range_from #n
   (#t: Type0)
@@ -47,11 +47,11 @@ val update_at_range_from #n
   (i: t_RangeFrom (int_t n))
   (x: t_Slice t)
   : Pure (t_Array t (length s))
-    (requires ( v i.f_start >= 0 /\ v i.f_start <= Seq.length s /\
-                Seq.length x == Seq.length s - v i.f_start))
+    (requires ( v i.f_start >= 0 /\ v i.f_start <= FStar.List.Tot.length s /\
+                FStar.List.Tot.length x == FStar.List.Tot.length s - v i.f_start))
     (ensures (fun res ->
-                Seq.slice res 0 (v i.f_start) == Seq.slice s 0 (v i.f_start) /\
-                Seq.slice res (v i.f_start) (Seq.length res) == x))
+                Rust_primitives.Arrays.list_slice res 0 (v i.f_start) == Rust_primitives.Arrays.list_slice s 0 (v i.f_start) /\
+                Rust_primitives.Arrays.list_slice res (v i.f_start) (FStar.List.Tot.length res) == x))
 
 val update_at_range_full
   (#t: Type0)
@@ -59,5 +59,5 @@ val update_at_range_full
   (i: t_RangeFull)
   (x: t_Slice t)
   : Pure (t_Array t (length s))
-    (requires (Seq.length x == Seq.length s))
+    (requires (FStar.List.Tot.length x == FStar.List.Tot.length s))
     (ensures (fun res -> res == x))
