hax-lib/proof-libs/fstar/rust_primitives/Rust_primitives.Hax.fst
@@ -6,8 +6,8 @@ open Rust_primitives.Arrays
 type t_Never = False
 let never_to_any #t: t_Never -> t = (fun _ -> match () with)
 
-let repeat #a (x: a) (len: usize): t_Array a len = 
-  FStar.Seq.create (v len) x
+let repeat #a (x: a) (len: usize): t_Array a len =
+  list_create (v len) x
 
 open Core_models.Ops.Index
 class update_at_tc self idx = {
@@ -27,26 +27,26 @@ instance impl__index_refined t l r: t_Index (t_Array t l) (x: usize {r x})
   = { f_Output = t;
       f_index_pre = (fun (s: t_Array t l) (i: usize {r i}) -> v i >= 0 && v i < v l);
       f_index_post = (fun _ _ _ -> true);
-      f_index = (fun s i -> Seq.index s (v i));
+      f_index = (fun s i -> FStar.List.Tot.index s (v i));
     }
 
 /// Similarly to `impl__index_refined`, we need to define a instance
 /// for refined `usize`.
 instance update_at_tc_array_refined t l r: update_at_tc (t_Array t l) (x: usize {r x}) = {
   super_index = impl__index_refined t l r;
-  update_at = (fun arr i x -> FStar.Seq.upd arr (v i) x);
+  update_at = (fun arr i x -> list_upd arr (v i) x);
 }
 
 instance impl__index t l: t_Index (t_Array t l) (usize)
   = { f_Output = t;
       f_index_pre = (fun (s: t_Array t l) (i: usize) -> v i >= 0 && v i < v l);
       f_index_post = (fun _ _ _ -> true);
-      f_index = (fun s i -> Seq.index s (v i));
+      f_index = (fun s i -> FStar.List.Tot.index s (v i));
     }
 
 instance update_at_tc_array t l: update_at_tc (t_Array t l) (usize) = {
   super_index = FStar.Tactics.Typeclasses.solve <: t_Index (t_Array t l) (usize);
-  update_at = (fun arr i x -> FStar.Seq.upd arr (v i) x);
+  update_at = (fun arr i x -> list_upd arr (v i) x);
 }
 
 
@@ -97,40 +97,60 @@ unfold let array_of_list (#t:Type)
   (n: nat {n < maxint U16})
   (l: list t {FStar.List.Tot.length l == n})
   : t_Array t (sz n)
-  = Seq.seq_of_list l
+  = l
 
 (* class iterator_return (self: Type u#0): Type u#1 = {
   [@@@FStar.Tactics.Typeclasses.tcresolve]
   parent_iterator: Core_models.Iter.Traits.Iterator.t_Iterator self;
   f_fold_return: #b:Type0 -> s:self -> b -> (b -> i:parent_iterator.f_Item{parent_iterator.f_contains s i} -> Core_models.Ops.Control_flow.t_ControlFlow b b) -> Core_models.Ops.Control_flow.t_ControlFlow b b;
 } *)
-let while_loop #acc_t 
+let while_loop #acc_t
   (inv: acc_t -> Type0)
-  (condition: (c:acc_t {inv c}) -> bool) 
+  (condition: (c:acc_t {inv c}) -> bool)
   (fuel: (a:acc_t{inv a} -> nat))
-  (init: acc_t {inv init}) 
-  (f: (i:acc_t{inv i /\ condition i} -> o:acc_t{inv o /\ fuel o < fuel i})): 
+  (init: acc_t {inv init})
+  (f: (i:acc_t{inv i /\ condition i} -> o:acc_t{inv o /\ fuel o < fuel i})):
   (res: acc_t {inv res /\ not (condition res)})
-  = 
+  =
   let rec while_loop_internal
-  (current: acc_t {inv current}): 
+  (current: acc_t {inv current}):
   Tot (res: acc_t {inv res /\ not (condition res)}) (decreases (fuel current))
   = if condition current
-    then 
-      let next = f current in 
+    then
+      let next = f current in
       assert (fuel next < fuel current);
       while_loop_internal next
-    else current in 
+    else current in
   while_loop_internal init
 
-assume val while_loop_return #acc_t #ret_t 
+let rec while_loop_return_aux (#acc_t #ret_t: Type0)
+  (condition: acc_t -> bool)
+  (fuel: acc_t -> nat)
+  (acc: acc_t)
+  (f: acc_t -> Core_models.Ops.Control_flow.t_ControlFlow
+    (Core_models.Ops.Control_flow.t_ControlFlow ret_t (Prims.unit & acc_t)) acc_t)
+  : Tot (Core_models.Ops.Control_flow.t_ControlFlow ret_t acc_t) (decreases (fuel acc))
+  = if not (condition acc) then Core_models.Ops.Control_flow.ControlFlow_Continue acc
+    else match f acc with
+    | Core_models.Ops.Control_flow.ControlFlow_Break (Core_models.Ops.Control_flow.ControlFlow_Break ret) ->
+        Core_models.Ops.Control_flow.ControlFlow_Break ret
+    | Core_models.Ops.Control_flow.ControlFlow_Break (Core_models.Ops.Control_flow.ControlFlow_Continue ((), acc')) ->
+        Core_models.Ops.Control_flow.ControlFlow_Continue acc'
+    | Core_models.Ops.Control_flow.ControlFlow_Continue acc' ->
+        if fuel acc' < fuel acc
+        then while_loop_return_aux condition fuel acc' f
+        else Core_models.Ops.Control_flow.ControlFlow_Continue acc'
+
+let while_loop_return #acc_t #ret_t
   (inv: acc_t -> Type0)
-  (condition: (c:acc_t {inv c}) -> bool) 
+  (condition: (c:acc_t {inv c}) -> bool)
   (fuel: (a:acc_t -> nat))
-  (init: acc_t ) 
-  (f: (acc_t -> Core_models.Ops.Control_flow.t_ControlFlow 
+  (init: acc_t)
+  (f: (acc_t -> Core_models.Ops.Control_flow.t_ControlFlow
   (Core_models.Ops.Control_flow.t_ControlFlow ret_t (Prims.unit & acc_t)) acc_t))
   : Core_models.Ops.Control_flow.t_ControlFlow ret_t acc_t
+  = let cond (a: acc_t): bool = assume (inv a); condition a in
+    while_loop_return_aux cond fuel init f
 
 /// Represents backend failures
 let failure #t (_error: string) (_ast: string): Pure t False (fun _ -> True) = ()
