hax-lib/proof-libs/fstar/rust_primitives/Rust_primitives.Iterators.fst
@@ -1,0 +1,87 @@
+module Rust_primitives.Iterators
+
+open Rust_primitives
+open Core_models.Ops.Range
+open FStar.Mul
+
+#set-options "--fuel 1 --ifuel 1 --z3rlimit 60"
+
+(* These functions are implemented with recursive helper + admit for postconditions.
+   The computation itself is correct; only the invariant proofs are admitted. *)
+
+let rec foldi_range_impl (#n:inttype) (#acc_t:Type)
+  (start end_: int_t n)
+  (acc: acc_t)
+  (f: acc_t -> int_t n -> acc_t)
+  : Tot acc_t (decreases (if v end_ > v start then v end_ - v start else 0))
+  = if v start >= v end_ then acc
+    else foldi_range_impl (start +! mk_int 1) end_ (f acc start) f
+
+let foldi_range #n #acc_t #inv r acc f =
+  admit ();
+  foldi_range_impl r.f_start r.f_end acc (fun a i -> f a i)
+
+let rec foldi_range_step_by_impl (#n:inttype) (#acc_t:Type)
+  (start end_: int_t n)
+  (step: nat {step > 0 /\ range step n /\ range (v end_ + step) n})
+  (acc: acc_t)
+  (f: acc_t -> int_t n -> acc_t)
+  : Tot acc_t (decreases (if v end_ > v start then v end_ - v start else 0))
+  = if v start >= v end_ then acc
+    else
+      let next_v = v start + step in
+      if next_v > v end_ then f acc start
+      else foldi_range_step_by_impl (mk_int #n next_v) end_ step (f acc start) f
+
+let foldi_range_step_by #n #acc_t #inv r step acc f =
+  admit ();
+  foldi_range_step_by_impl r.f_start r.f_end (v step) acc (fun a i -> f a i)
+
+let rec foldi_chunks_exact_impl
+  (#t #acc_t:Type)
+  (s: t_Slice t)
+  (chunk_len: nat {chunk_len > 0})
+  (acc: acc_t)
+  (f: acc_t -> (nat & list t) -> acc_t)
+  (i: nat)
+  : Tot acc_t (decreases (FStar.List.Tot.length s / chunk_len - i))
+  = if i >= FStar.List.Tot.length s / chunk_len then acc
+    else
+      let chunk = Rust_primitives.Arrays.list_slice s (chunk_len * i) (chunk_len * (i + 1)) in
+      foldi_chunks_exact_impl s chunk_len (f acc (i, chunk)) f (i + 1)
+
+let foldi_chunks_exact #t #acc_t #inv s chunk_len acc f =
+  admit ();
+  foldi_chunks_exact_impl s (v chunk_len) acc (fun a (i, c) -> f a (sz i, c)) 0
+
+let rec fold_chunks_exact_impl
+  (#t #acc_t:Type)
+  (s: t_Slice t)
+  (chunk_len: nat {chunk_len > 0})
+  (acc: acc_t)
+  (f: acc_t -> list t -> acc_t)
+  (i: nat)
+  : Tot acc_t (decreases (FStar.List.Tot.length s / chunk_len - i))
+  = if i >= FStar.List.Tot.length s / chunk_len then acc
+    else
+      let chunk = Rust_primitives.Arrays.list_slice s (chunk_len * i) (chunk_len * (i + 1)) in
+      fold_chunks_exact_impl s chunk_len (f acc chunk) f (i + 1)
+
+let fold_chunks_exact #t #acc_t #inv s chunk_len acc f =
+  admit ();
+  fold_chunks_exact_impl s (v chunk_len) acc (fun a c -> f a c) 0
+
+let rec foldi_slice_impl (#t #acc_t:Type)
+  (sl: list t)
+  (acc: acc_t)
+  (f: acc_t -> (nat & t) -> acc_t)
+  (i: nat)
+  : Tot acc_t (decreases (FStar.List.Tot.length sl - i))
+  = if i >= FStar.List.Tot.length sl then acc
+    else
+      let item = FStar.List.Tot.index sl i in
+      foldi_slice_impl sl (f acc (i, item)) f (i + 1)
+
+let foldi_slice #t #acc_t #inv sl acc f =
+  admit ();
+  foldi_slice_impl sl acc (fun a (i, item) -> f a (sz i, item)) 0
