hax-lib/proof-libs/fstar/rust_primitives/Rust_primitives.Slice.fsti
@@ -4,18 +4,18 @@ open FStar.Mul
 open Rust_primitives.Arrays
 open Rust_primitives.Integers
 
-let slice_length (#a: Type) (s: t_Slice a): res: usize {res == sz (Seq.length s)} = sz (Seq.length s)
-let slice_split_at (#v_T: Type0) (s: t_Slice v_T) (mid: usize {mid <=. length s}): t_Slice v_T & t_Slice v_T = 
-  Seq.slice s 0 (v mid), Seq.slice s (v mid) (Seq.length s)
-let slice_contains (#a: eqtype) (s: t_Slice a) (v: a): bool = Seq.mem v s
-let slice_index (#t: Type) (s: t_Slice t) (i: usize {i <. length s}): t = Seq.index s (v i)
+let slice_length (#a: Type) (s: t_Slice a): res: usize {res == sz (FStar.List.Tot.length s)} = sz (FStar.List.Tot.length s)
+let slice_split_at (#v_T: Type0) (s: t_Slice v_T) (mid: usize {mid <=. length s}): t_Slice v_T & t_Slice v_T =
+  list_slice s 0 (v mid), list_slice s (v mid) (FStar.List.Tot.length s)
+let slice_contains (#a: eqtype) (s: t_Slice a) (v: a): bool = FStar.List.Tot.mem v s
+let slice_index (#t: Type) (s: t_Slice t) (i: usize {i <. length s}): t = FStar.List.Tot.index s (v i)
 let slice_slice (#v_T: Type0) (s: t_Slice v_T) (start: usize {start <=. length s}) (end_: usize {start <=. end_ /\ end_ <=. length s}): t_Slice v_T =
-  Seq.slice s (v start) (v end_)
+  list_slice s (v start) (v end_)
 val array_map (#t: Type) (#u: Type) (l: usize) (#ft: Type)
-  (s: t_Array t l) (f: t -> u): res: t_Array u l {forall i. Seq.index res i == f (Seq.index s i)}
+  (s: t_Array t l) (f: t -> u): res: t_Array u l {forall i. FStar.List.Tot.index res i == f (FStar.List.Tot.index s i)}
 let array_as_slice (#t: Type) (l: usize) (s: t_Array t l): t_Slice t =
   s
 let array_slice (#t: Type) (l: usize) (s: t_Array t l) = slice_slice s
-val array_from_fn (#t: Type) (len: usize) (#ft: Type) (f: (x: usize {x <. len}) -> t): 
-  Pure (t_Array t len) (requires True) (ensures (fun a -> forall i. Seq.index a i == f (sz i)))
-let array_index (#t: Type) (l: usize) (s: t_Array t l) (i: usize {i <. length s}): t = Seq.index s (v i)
+val array_from_fn (#t: Type) (len: usize) (#ft: Type) (f: (x: usize {x <. len}) -> t):
+  Pure (t_Array t len) (requires True) (ensures (fun a -> forall i. FStar.List.Tot.index a i == f (sz i)))
+let array_index (#t: Type) (l: usize) (s: t_Array t l) (i: usize {i <. length s}): t = FStar.List.Tot.index s (v i)
